# Hasse-Weil Theorem

$p$ prime, $q = pâ¿$
$$ \Phi : \bar{ğ”½}_q â†’ \bar{ğ”½}_q = \bar{ğ”½}_p = \bigcup_n ğ”½_{pâ¿} $$
$$ \Phi(x) = x^q $$
it is a field homomorphism.
Induces a map for $E/ğ”½_q$
$$ \Phi: E(\bar{ğ”½}_q) â†’ E(\bar{ğ”½}_q) $$
$$ \Phi(x, y) = (x^q, y^q) $$
Frobenius is compatible wih group structure on $E(\bar{ğ”½}_q)$.

## Definition: Isogeny

$E, E'$ are EC on $K$. An isogeny $Î± : E â†’ E'$ is a rational map
such that the induced map
$$ E(\bar{K}) â†’ E'(\bar{K}) $$
is a group homomorphism

## Example: Frobenius

## Isogeny $Î± : E â†’ E$ is an endomorphism.

If $Î± : E/K â†’ E'/K$ is an isogeny then
$$ Î± : E(L) â†’ E'(L) $$
for $K âŠ† L âŠ† \bar{K}$ is an isogeny.
$$ E(L) âŠ† E(\bar{K}) $$

## Example

Let $E/K$ be any EC, for all $n$ multiplication by $n$
is an endomorphism.
$$ [n] : E â†’ E $$
$$ P â†’ nP $$
Everything we do is polynomials and it preserves group structure.

## Recall:

An isogeny $Î± : E â†’ E'$ viewed as a rational map, has a canonical form.
$$ Î±(x, y) = (râ‚(x), yrâ‚‚(x)) $$
where $rÙâ‚(x) = \frac{p(x)}{q(x)}, râ‚‚(x) = \frac{u(x)}{v(x)}$
and each quotient is reduced, so no common factors over $\bar{K}$.

If $q(x) = 0$ for some $x, y âˆˆ E(\bar{K})$, then we set $Î±(x, y) = 0_{E'}$
and otherwise we showed $v(x) â‰  0$ and hence $Î±$ is well defined.

## Def

Let $Î± : E/K â†’ E'/K$ be an isogeny.

1. The degree of $Î±$ is $\deg(Î±) = \textrm{max}\{ \deg(p), \deg(q) \}$.
2. $Î±$ is called separable if the formal derivative $râ‚'(x)$ is not identically
   zero â‡”  $p(x) q'(x) - p'(x) q(x) â‰  0$

$$ \Phi_q = Î± : E(\bar{ğ”½}_q) â†’ E(\bar{ğ”½}_q) $$
$$ âˆ â†’ âˆ $$
$$ (x, y) â†’ (x^q, y^q) âˆˆ E(\bar{ğ”½}_q) $$
$$ (y^q)Â² = (x^q)Â³ + Ax^q + B $$
$$ (yÂ²)^q = (xÂ³ + Ax + B)^q $$

Is $\Phi_q$ separable?
$$ (x^q)' = qx^{q - 1} = 0 \textrm{ in } ğ”½_q $$
so it is not separable.

## Prop

Let $Î± : E â†’ E'$ be a nonzero isogeny.
If $Î±$ is separable then
$$ \# \textrm{ker}(Î± : E(\bar{K}) â†’ E'(\bar{K})) = \deg(Î±) $$
and otherwise $\#\textrm{ker}(Î±) < \deg(Î±)$

### Observe $\# E(ğ”½_q) = \# \ker(Î±)$

For $E/ğ”½_q$
$$ Î± : \Phi^n_q - \textrm{id} : E â†’ E $$
$$ P â†’ \Phi_q^n(P) - P $$
$$ \ker(Î± : E(\bar{ğ”½}_q) â†’ E(\bar{ğ”½}_q)) = \# E(ğ”½_{q^n}) $$

(or without $n$ easier)

For $E/ğ”½_q$
$$ Î± : \Phi_q - \textrm{id} : E â†’ E $$
$$ P â†’ \Phi_q(P) - P $$
$$ \ker(Î± : E(\bar{ğ”½}_q) â†’ E(\bar{ğ”½}_q)) = \# E(ğ”½_{q}) $$
$$P âˆˆ \ker(Î±) â‡” \Phi_q(P) -P = âˆ $$
$$ â‡” \Phi_q(P) = P $$
we saw that these points $P$ are exactly $E(ğ”½_q)$

The only points frobenius acts as identity is those in $ğ”½_q$,
so only unchanged points are in the kernel.
In higher extensions, frobenius doesn't act as the identity.

## Proof

Since $Î± â‰  0$ and is a group homomorphism on $E(\bar{K}) â†’ E'(\bar{K})$
it is non-constant.

Thus $Î± : E(\bar{K}) â†’ E'(\bar{K})$ is surjective. Let $Q = (a, b) âˆˆ E'(\bar{K})$
and $P = (xâ‚€, yâ‚€) âˆˆ E(\bar{K})$.

## Exercise: Show the prop on surjectivity generalizes to the case of $E â†’ E'$

Since $E'(\bar{K})$ is infinite we can choose $Q$ st

1. $a, b â‰  0$
2. $\deg(p - qa) = \max\{\deg(p), \deg(q) \} = \deg(Î±)$

the only case in which $\deg(p - qa) < \deg(Î±)$ is when
$\deg(p) = \deg(q)$ and their leading coefficients $Î», Î´$ respectively
satisfy
$$ Î» - aÎ´ = 0 â‡” a = \frac{Î»}{Î´} $$
so we choose $Q$ such that $a â‰  \frac{Î»}{Î´}$.

Since $\deg(p - aq) = \deg(Î±)$,
$p(x) - aq(x)$ has exactly $\deg(Î±)$ roots over $\bar{K}$
(possibly repeated roots).

We claim that the number of distinct roots of $p - aq$ is exactly the
number of sources $P$ of $Q$ (under $Î±$).

Since $(a, b) â‰  (âˆ, âˆ)$, then
$$râ‚(xâ‚€) â‰  0 â‡” q(xâ‚€) â‰  0$$
since $b â‰  0$ and we have
$$yâ‚€ râ‚‚(x) = b$$
we have $yâ‚€ = b / râ‚‚(xâ‚€)$, so $yâ‚€$ is completely determined by $xâ‚€$.

So it is enough to count the $xâ‚€$'s which in turn must satisfy
$\frac{p(xâ‚€)}{q(xâ‚€)} = a$
$$ â‡” p(xâ‚€) - aq(xâ‚€) = 0 $$
i.e the roots of $p - aq$

Since $Î±$ is a group homomorphism on $E(\bar{K}) â†’ E'(\bar{K})$,
then $\# \ker(Î±)$ is the same as the number of sources of any given
point $Q âˆˆ E'(\bar{K})$

Which is enough to analyze the number of distinct roots $xâ‚€$ of $p - aq$.

$xâ‚€$ is a repeated root of $p - aq â‡”  p(xâ‚€) - aq(xâ‚€) = 0$
and also $p'(xâ‚€) - aq'(xâ‚€) = 0$.
Multiply both equations to get
$$ap(xâ‚€)q'(xâ‚€) = ap'(xâ‚€)q(xâ‚€)$$
Since $a â‰  0$
$$p(xâ‚€)q'(xâ‚€) - p'(xâ‚€)q(xâ‚€) = 0$$
$$râ‚'(xâ‚€) = 0 $$
by the quotient rule applied to $râ‚'$.

If $Î±$ is not separable
$$ râ‚'(x) = 0 $$
which means $p - aq$ has repeated roots
and $\# \ker(Î±) < \deg(Î±)$.

If $Î±$ is separable
$$ râ‚'(x) â‰  0 $$
and hence has a finite number of roots $S$.
We may add a constraint on the choice of $Q$
saying that $a âˆ‰ râ‚(S)$. Then since
$râ‚(xâ‚€) = a$
$$xâ‚€ âˆ‰ S$$
so $p - aq$ will not have repeated roots,
i.e. $\# \ker(Î±) = \deg(Î±)$.

$$ râ‚'(x) = \frac{ p(x)q'(x) - q'(x)p(x) }{ q(x)Â² } $$

# Weil Pairing

Recall $\textrm{gcd}(n, \textrm{char} K) = 1$.
For $Q âˆˆ E[n]$ take $f_Q âˆˆ K(E) : \textrm{div}(f_Q) = n[Q] - n[âˆ]$,
there exists $g_Q âˆˆ K(E) : \textrm{div}(g_Qâ¿) = \textrm{div}(f_Q \circ [n])$.

For arbitrary $S âˆˆ E(K), P âˆˆ E[n]$
$$ e_n(P, Q) = \frac{ g_Q(S + P) }{ g_Q(S) } $$
(this does not depend on the choice of $S$)
$$ e_n : E[n] Ã— E[n] â†’ Î¼_n(K) $$

## $e_n(Î±(P), Î±(Q)) = e_n(P, Q)^{\deg Î±}$

Let $Î± : E â†’ E$ be a separable endomorphism.

Observe that $Î±(P), Î±(Q) âˆˆ E[n]$ since
$$ n Î±(P) = Î±(nP) = Î±(âˆ) = âˆ $$

Let $\{ Tâ‚, â€¦, T_k \} = \ker (Î±)$. Since $Î±$ is separable, $k = \deg(Î±)$.

$$ \textrm{div}(f_Q) = n[Q] - n[âˆ] $$
$$ \textrm{div}(f_{Î±(Q)}) = n[Î±(Q)] - n[âˆ] $$
$$ g_Qâ¿ = f_Q \circ [n] $$
$$ g_{Î±(Q)}â¿ = f_{Î±(Q)} \circ [n] $$

Let $Ï„_T : E â†’ E$ be $X â†’ X + T$ translation by $T$.

Then $\textrm{div}(f_Q \circ Ï„_{-T_i}) = n[Q + T_i] - n[T_i]$.

Now notice that $\textrm{div}(f_{Î±(Q)}) = n[Î±(Q)] - n[âˆ]$ and so
\begin{align*}
\textrm{div}(f_{Î±(Q)} \circ Î±) &= n \sum_{Q'' : Î±(Q'') = Î±(Q)} [Q''] - n \sum_{T : Î±(T) = âˆ} [T] \\
        &= n \sum_{i = 1}^k ([Q + T_i] + [T_i]) \\
        &= \textrm{div}(\prod_{i = 1}^k f_Q \circ Ï„_{-T_i})
\end{align*}

For $1 â‰¤ i â‰¤ k$ choose $T_i' âˆˆ E[nÂ²] : nT_i' = T_i$ then
\begin{align*}
g_Q(S - T_i')â¿ &= f_Q \circ [n](S - T_i') \\
    &= f_Q(nS - T_i)
\end{align*}
by the definition of $g_Q$.

Now using this identity, we can see that
\begin{align*}
\textrm{div}( \prod_{i = 1}^k (g_Q \circ Ï„_{-T_i'})â¿) &=
    \textrm{div}( \prod_{i = 1}^k f_Q \circ Ï„_{-T_i} \circ [n] ) \\
    &= \textrm{div}( f_{Î±(Q)} \circ Î± \circ [n] )
\end{align*}
where we use the expression from above for $\textrm{div}(f_{Î±(Q)} \circ Î±)$.

Notice $Î± \circ [n] = [n] \circ Î±$ because $nÎ±(P) = Î±(nP)$, so multiplication
by $n$ commutes with endormorphisms.
\begin{align*}
    \textrm{div}( f_{Î±(Q)} \circ Î± \circ [n] )
    &= \textrm{div}( f_{Î±(Q)} \circ [n] \circ Î± ) \\
    &= \textrm{div}( (g_{Î±(Q)}â¿) \circ Î±) \\
    &= \textrm{div}( (g_{Î±(Q)} \circ Î±)â¿ )
\end{align*}

Finally we get
$$ \prod_{i = 1}^k (g_Q \circ Ï„_{-T_i'}) = g_{Î±(Q)} \circ Î± $$

\begin{align*}
e_n(Î±(P), Î±(Q)) &= \frac{ g_{Î±(Q)}(Î±(P) + Î±(S)) }{ g_{Î±(Q)}(Î±(S)) } \\
    &= \prod_{i = 1}^k \frac{
        g_Q(P + S - T_i')
    }{
        g_Q(S - T_i')
    } \\
    &= \prod_{i = 1}^k e_n(P, Q) = e_n(P, Q)^k \\
    &= e_n(P, Q)^{\deg Î±}
\end{align*}

# General Direction

\begin{align*}
\# E(ğ”½_q) &= \# \ker (\Phi_q - \textrm{id}) \\
          &= \deg (\Phi_q - \textrm{id})
\end{align*}
then we can estimate this degree.

# Separable Map

Definition of separable map
$$ \deg Î± = \# \ker(Î±) $$
alternatively $râ‚'(x) â‰  0$.

$P, Q âˆˆ E[n]$ and $Î±$ is separable then
$e_n(Î±(P), Î±(Q)) = e_n(P, Q)^{\deg Î±}$.

# Invariance of Weil Pairing under "action of Galois group"

$$ \textrm{Gal}(\bar{K}/K) = \{ Ïƒ âˆˆ \textrm{Aut}(\bar{K}) : Ïƒ|_k = \textrm{id}_K \}$$

$$ \Phi_q âˆˆ \textrm{Gal}(\bar{ğ”½}_q / ğ”½_q) $$

## Proposition

$$ Ïƒ âˆˆ \textrm{Gal}(\bar{ğ”½}_q / ğ”½_q) $$

$$ Ïƒ(e_n(P, Q)) = e_n(ÏƒP, ÏƒQ) $$

Note $ÏƒP âˆˆ E$ since $Ïƒ(y)Â² = Ïƒ(x)Â³ + AÏƒ(x) + B$, and
then adding is rational so $P âˆˆ E[n] â‡’ n Â· ÏƒP = âˆ$.

Recall that $f_Q, g_Q âˆˆ K(E)$
$$ \textrm{div}(f_Q) = n[Q] - n[âˆ] $$
and $g_Q$ that satisfy
$$ g_Qâ¿ = f_Q \circ [n] $$
and for any $S âˆˆ E(K)$
$$ e_n(P, Q) = \frac{ g_Q(P + S) }{ g_Q(S) } $$

Write out $f_Q$ and then when it equals zero, applying $Ïƒ$ you see
that $ÏƒQ$ is now a root of $f_Q^Ïƒ$, so
$$\textrm{div}(f_Q^Ïƒ) = n[ÏƒQ] - n[âˆ]$$
and similarly for $g_Q^Ïƒ$.

\begin{align*}
(g_Q^Ïƒ)â¿ &= (g_Qâ¿)^Ïƒ \\
        &= (f_Q \circ [n])^Ïƒ \\
        &= f_Q^Ïƒ \circ [n]
\end{align*}

Thus
\begin{align*}
Ïƒ(e_n(P, Q)) &= Ïƒ(\frac{g_Q(P + S)}{g_Q(S)}) \\
    &= \frac{ g_Q^Ïƒ(ÏƒP + ÏƒS) } { g_Q^Ïƒ(ÏƒS) } \\
    &= e_n(ÏƒP, ÏƒQ)
\end{align*}

Where the last step comes from the construction of the Weil pairing.
Namely $g_Q^Ïƒ = g_{ÏƒQ}$.
\begin{align*}
(g_{ÏƒQ})â¿ &= f_{ÏƒQ} \circ [n] \\
    &= f_Q^Ïƒ \circ [n] \\
    &= (g_Qâ¿)^Ïƒ \\
    &= (g_Q^Ïƒ)â¿ \\
    &= (f_Q \circ [n])^Ïƒ \\
    &= f_Q^Ïƒ \circ [n]
\end{align*}

# Restriction of $Î±$ to $E[n]$ stays in $E[n]$

$$ E[n] = â„¤_n Ã— â„¤_n $$
so $E[n] = âŸ¨Tâ‚, Tâ‚‚âŸ©$.
$$ Î±_n =
\begin{pmatrix}
a & b \\
c & d \\
\end{pmatrix}
$$
\begin{align*}
Î±(Tâ‚) &= aTâ‚ + cTâ‚‚ \\
Î±(Tâ‚‚) &= bTâ‚ + dTâ‚‚ \\
Î±(P) &= Î±(rTâ‚ + sTâ‚‚) \\
    &= rÎ±(Tâ‚) + sÎ±(Tâ‚‚)
\end{align*}
$$ P = rTâ‚ + sTâ‚‚ $$
$$
\begin{pmatrix}
a & b \\
c & d \\
\end{pmatrix}
\begin{pmatrix}
r \\
s \\
\end{pmatrix}
=
\begin{pmatrix}
x \\
y \\
\end{pmatrix}
$$
$$ Î±(P) = xTâ‚ + yTâ‚‚ $$

# $\det(Î±_n) = \deg(Î±) \textrm{mod} n$

By weil pairing property $e_n(Tâ‚, Tâ‚‚)$ maps to a generator
for $Î¼_n(ğ”½_q)$.
Let $Î· = e_n(Tâ‚, Tâ‚‚)$.
Since $Î±$ is separable of $\Phi_q$
$$ Î·^{\deg{(Î±)}} = e_n(Tâ‚, Tâ‚‚)^{\deg(Î±)} = e_n(Î±(Tâ‚), Î±(Tâ‚‚)) $$
But using the matrix we get
\begin{align*}
e_n(aTâ‚ + cTâ‚‚, bTâ‚ + dTâ‚‚) &= e_n(Tâ‚, Tâ‚)^{ab} e_n(Tâ‚, Tâ‚‚)^{ad} e_n(Tâ‚‚, Tâ‚)^{bc} e_n(Tâ‚‚, Tâ‚‚)^{cd} \\
&= 1^{ab} e_n(Tâ‚, Tâ‚‚)^{ad} e_n(Tâ‚‚, Tâ‚)^{bc} 1^{cd} \\
&= 1^{ab} e_n(Tâ‚, Tâ‚‚)^{ad} e_n(Tâ‚, Tâ‚‚)^{-bc} 1^{cd} \qquad \text{by pairing rule about swapping args}\\
&= e_n(Tâ‚, Tâ‚‚)^{ad - bc} \\
&= e_n(Tâ‚, Tâ‚‚)^{\det(Î±_n)} \\
&= Î·^{\det(Î±_n)}
\end{align*}
since $Î·$ is a generator, we must have
$$ \deg(Î±) â‰¡ \det(Î±_n) \mod n $$

# $\deg(aÎ± + bÎ²) = aÂ² \deg(Î±) + bÂ² \deg(Î²) + ab (\deg(Î± + Î²) - \deg(Î±) - \deg(Î²))$

Restrict $Î±, Î²$ using matrices $Î±_n, Î²_n$, where char $K \nmid n$.

Note from linear algebra matrix determinant rules
$\det(aÎ±_n + bÎ²_n) = aÂ² \det(Î±_n) + bÂ² \det(Î²_n) + ab (\det(Î±_n + Î²_n) - \det(Î±_n) - \det(Î²_n))$.

Now replace determinant by degree for mod n.

Since this is true for infinitely many n's, we have ordinary equality.

# $\deg(r \Phi_q + s) = rÂ² q + sÂ² - rst$

$r, s âˆˆ â„¤, \gcd(s, q) = 1$ then
$$t = q + 1 - \deg(\Phi_q - 1)$$
By previous proposition
$$ \deg(r\Phi_q - s) = rÂ² \deg(\Phi_q) + sÂ² \deg(-1) + rs(\deg(\Phi_q - 1) - \deg(\Phi_q) - \deg(-1)) $$
Since $\deg(\Phi_q) = q$ and $\deg(-1) = 1$
$$ \deg(r\Phi_q - s) = rÂ² q + sÂ² + rs(\deg(\Phi_q - 1) - q - 1) $$

# Hasse-Weil Theorem

$$ | q + 1 - \# E(ğ”½_q) | â‰¤ 2 \sqrt{q} $$

$$ \deg(\Phi_q - 1) = \# \ker(\Phi_q - 1) = \# E(ğ”½_q) $$

For any $r, s âˆˆ â„¤$ such that $\gcd(s, q) = 1$, we have
$$ 0 â‰¤ \deg(r \Phi_q - s) $$
because degrees are greater than 0.

$$ rÂ²q + sÂ² - rst >= 0 $$
$$ â‡” q(\frac{r}{s})Â² - t(\frac{r}{s}) + 1 â‰¥ 0 $$
The set of all rational numbers $r/s$ such that $\gcd(s, q) = 1$
is dense in $\mathbb{R}$ so the polynomial
$$ qxÂ² - tx + 1 $$
gets only non-negative values, and
has non-positive discriminant.
$$ tÂ² - 4q â‰¤ 0 $$

## Dense Set

If $\forall x âˆˆ \mathbb{R}$, there exists a sequence
$$ s_1, s_2, â€¦, s_n, â€¦ $$
$$ \lim_{n â†’ âˆ} s_n = x $$

For example $\pi$ can be approximated with an infinite sequence of rationals.

Take $xâ‚€ âˆˆ \mathbb{R}$ since there exists a sequence $Ïƒ_n = r_n / s_n$
such that $\lim Ïƒ_n = x_0$.

$$ 0 â‰¤ \lim_{n â†’ âˆ}(q Ïƒ_nÂ² - tÏƒ_n + 1) = q(\lim_{n â†’ âˆ})Â² - t \lim_{n â†’ âˆ}(Ïƒ_n) + 1 $$
$$ â‡’ qxâ‚€Â² - txâ‚€ + 1 â‰¥ 0 $$

# Hasse-Weil Corrollary

In End($E$)
$$ \Phi_q^2 - [t] \circ \Phi_q + [q] = 0 $$

For all $p \nmid n$
$$ E[n] \cong â„¤_n Ã— â„¤_n $$
so we represent $\Phi_q |_{E[n]} : E[n] â†’ E[n]$
as a matrix 
$A = \begin{pmatrix}
a & b \\
c & d \\
\end{pmatrix}$ (choose generators $\{T_1, T_2\} âŠ† E[n]$ which correspond to
$\{ (1, 0), (0, 1)\} âˆˆ â„¤_n Ã— â„¤_n$)

Any $2x2$ satisfies
$$ AÂ² - \textrm{tr}(A Â· A) + \det(AÂ·I) = 0 $$
where $\textrm{tr}(A) = a + d$.

We showed that
$$\det(A_n) = \deg(\Phi_n) \mod n $$
and another direct calc shows
$$ \textrm{tr}(A_n) = 1 + \det(A_n) = \det(I - A_n) $$
thus
\begin{align*}
\textrm{tr}(A_n) &= 1 + \deg \Phi_q + \deg(\textrm{id} - \Phi_q) \\
    &= 1 + \deg \Phi_q + \deg(\Phi_q - \textrm{id}) \\
    &= 1 + q - (q + 1 - t) \mod n \\
    &= t \mod n
\end{align*}
substititng, we get
$$ AÂ² - tÂ·A + qÂ·I = 0 $$
Now since this is true for infinitely many n,
it should be true in End($E$) $â‡’$
$$ \Phi_qÂ² + [t]Â·\Phi_q + [q] = 0 $$

