---
title: Homo Algebra by Rotman, Chapter 3
header-includes: |
    - \DeclareMathOperator\ker{ker}
    - \DeclareMathOperator\im{im}
    - \DeclareMathOperator\Frac{Frac}
    - \newcommand{\Hom}{\textrm{Hom}}
    - \newcommand{\rmod}{{}_R \textrm{Mod}}
    - \newcommand{\modr}{\textrm{Mod}_R}
---

# Projective Modules Split Exact Sequences

## $P$ is projective $⟹$ every $0 → A → B → P → 0$ splits

\begin{tikzcd}
         &          &          & P \ar[d, "1_P"] \ar[dl, dotted] & \\
0 \ar[r] & A \ar[r] & B \ar[r] & P \ar[r] & 0
\end{tikzcd}
we induce $j : P → B$ with $1_P = pj$ so that $P$ is a retract of $B$.

## Every $0 → A → B → P → 0$ splits $⟹ P$ is projective

We can construct an exact sequence which splits by the hypothesis,
then we have the projective map.

\begin{tikzcd}
0 \ar[r] & Rᵐ \ar[r] & Rⁿ \ar[r, shift left=1] \ar[d, dotted] & P \ar[r] \ar[d]
    \ar[l, shift left=1] & 0 \\
         &           & B  \ar[r]                & C \ar[r]               & 0
\end{tikzcd}

Let $A$ be a submodule of $B ∈ \rmod$. If $B/A$ is projective, then
$B = A ⊕ B/A$.

# $P$ is Projective $⟺$ $P$ is a Direct Summand of a Free Module

$$ 0 → \ker g → F → P → 0 $$

# Projective Basis

$A ∈ \rmod$ is projective $⟺ ∃ (aᵢ ∈ A)_{i ∈ I}$ and $(𝜙ᵢ : A → R)_{i ∈ I}$
such that $∀x ∈ A$, we have $x = \sum_{i ∈ I} (𝜙ᵢx)aᵢ$.

Also $A = ⟨(aᵢ)⟩$.

Let $A$ be projective, then $ψ : F → A$ with $𝜙$ by split property.

Define $aᵢ = ψ(eᵢ)$. For $x ∈ A$, then 
$$ 𝜙(x) = r₁e₁ + ⋯ + rₙeₙ $$
Define $𝜙ᵢ(x) = rᵢ$, then
$$ x = (𝜙₁x)a₁ + ⋯ + (𝜙ₙx)aₙ $$

For the converse, let there be
$(aᵢ ∈ A)_{i ∈ I}$ and $(𝜙ᵢ : A → R)_{i ∈ I}$.
Define $ψ : F → A$ by $ψ(eᵢ) = aᵢ$. Define $𝜙(x) = (𝜙₁x)e₁ + ⋯ + (𝜙ₙx)eₙ$
then $ψ𝜙 = 1$. So $A$ is a direct summand of $F$ and therefore projective.

# Schanuel's Lemma

$$ 0 → K → P → M → 0 $$
$$ 0 → K' → P' M → 0 $$
with $P, P'$ projective
$$ ⟹  K ⊕ P' ≌ K' ⊕ P $$

\begin{tikzcd}
0 \ar[r] & K \ar[r, "i"] \ar[d, dotted, "α"] & P \ar[r] \ar[d, dotted, "β"] & M \ar[r] \ar[d, "1_M"] & 0 \\
0 \ar[r] & K' \ar[r, "i'"]       & P' \ar[r]       & M \ar[r] & 0
\end{tikzcd}

Since P is projective, we induce the middle map $P → P'$. Then we get the
left one for free.

Now we use this to construct
\begin{tikzcd}
0 \ar[r] & K \ar[r, "θ"] & P ⊕ K' \ar[r, "ψ"] & P' \ar[r] & 0
\end{tikzcd}
which splits since $P'$ is projective.
$$ θ(x) = (ix, αx) $$
$$ ψ(u, x') = βu - i'x' $$

# Proposition 3.18/Corollary 3.19: Noetherian

## Submodules remain finitely generated of left noetherian modules

*Let $R$ be left noetherian, and $M ∈ \rmod$ be finitely generated.
Then every submodule is finitely generated.*

If $n = 1$, then $M = ⟨m⟩ ≌ R/I$ for some ideal. Let $S ⊆ M$ be the submodule,
then $S ≌ J/I$ for some ideal $I ⊆ J ⊆ R$. Since $R$ is left noetherian, this
means $J$ and hence $J/I$ is finitely generated, and so is $S$.

Now let $n ≥ 1$ with $M = ⟨x₁, …, xₙ, xₙ₊₁⟩$ and $M' = ⟨x₁, …, xₙ⟩$.
$$ 0 → M' → M → M'' = M/M' → 0 $$
$M'' = ⟨xₙ + M'⟩$ is cyclic. Let $S ⊆ M$ be the submodule, then
$$ 0 → S ∩ M' → S → S/(S∩M') → 0 $$
Given any sequence $0 → A → B → C → 0$, if $A$ and $C$ are finitely generated,
then so is $B$.

$S ∩ M' ⊆ M'$ and so is finitely generated. $S/(S∩M') ≌ (S + M')/M' ⊆ M/M'$ and
so is also finitely generated. Thus $S$ is finitely generated.

## Left noetherian module over PID ring generated by $n$ or fewer elements

For the base step $n = 1$, $M$ is therefore cyclic, and $J$ is PID by
hypothesis, so that $J/I$ is cyclic too.

Same as above, but use that if $A$ and $C$ are generated by $m$ and $n$
elements, then $B$ is generated by $m + n$ elements (or less).

## $M ∈ \rmod$ where $R$ is left noetherian is finitely presented

$𝜙 : F → M$ is surjective, then by above all submodules including $\ker 𝜙$
are finitely generated.

# Baer's Criterion

Use Zorn's lemma with partially ordered pairs fixing the previous item.
The maximal element is $(A₀, g₀)$. So there's a $b ∈ B : b ∉ A₀$.

Let $I = \{ r : rb ∈ A₀ \}$. This is an ideal since $A₀$ is a submodule.
It is all multiples of $b$ that are in $A₀$. But there are some primitive
multiples (and their factors) that remain outside $A₀$.
Define the map $h : I → E$
$$ h(r) = g₀(rb) $$
By the hypothesis, this extends to $h^* : R → E$.
Then we can extend $A₁ = A₀ + ⟨b⟩$ and make $g₁ : A → E$ by
$g₁(a₀ + rb) = g₀(a₀) + rh^*(1)$.
We can see $gِ₁$ extends $g₀$ which contradicts the maximality of $(A₀, g₀)$.

Now for the final step, we must just prove that $g₁$ is well defined.
Let $a₀ + rb = a₀' + r'b$.

* $(r - r')b = a₀' - a₀ ∈ A₀ ⟹ r - r' ∈ I$.
* Thus $g₀((r - r')b)$ and $h(r - r')$ are defined.
* $g₀((r - r')b) = (r - r')h^*(1) ⟹ g₀(r) + rh^*(1) = g₀(r') + r'h^*(1)$

So even if there are multiple ways of writing an element as $a₀ + rb$
then applying $g₁$ always gives the same result.

#

* Direct product of injective modules is injective.
* If $R$ is left noetherian, then direct sum of injective R-modules is
  injective.
* If $R$ is a domain then every injective R-module is divisible.
* If $R$ is a domain, then $\Frac(Q)$ is an injective $R$-module.
* If $R$ is PID, then $E$ is injective $⟺ E$ is divisible.
* If $R$ is PID, then every quotient of injective modules are injective.
* If $D$ is a divisible abeligan group, then $\Hom_ℤ(R, D)$ is an injective
  left $R$-module.

# Every Module Can be Embedded in an Injective Module

This means injective sequences split since we can construct
$0 → M'' → M → E → 0$ where $M$ is injective.

# $E ∈ \rmod$ is Injective $⟺$ every $0 → E → B → C → 0$ where $C$ is Cyclic Splits

$E$ is injective $⟹$ every sequence splits, so we only need to prove the
converse.

Let $I$ be an ideal of $R$, and let $f : I → E$. By category (see prev lemma
3.41), we can construct this diagram:
\begin{tikzcd}
0 \ar[r] & I \ar[d] \ar[r] & R \ar[d] \ar[r] & R/I \ar[d, "1_{R/I}"] \ar[r] & 0 \\
0 \ar[r] & E        \ar[r] & P        \ar[r] & R/I        \ar[r] & 0
\end{tikzcd}

Since $R/I$ is cyclic, by hypothesis the bottom row splits.

Thus there's a map $P → E$ which we compose with $R → P$ to get $R → E$, then
by Baer's criterion, we have shown $E$ is injective.

# Flat Modules

* $R$ is a flat $R$-module.
* Direct sums are flat, and flat direct sums means all their submodules are
  flat.
* Projective modules are flat.
* Let $0 → A → B$ and $u ∈ \ker(1⊗i)$. Then there is a finitely generated
  $N ⊆ M$ and $u' ∈ N⊗A$ such that:
    * $u' ∈ \ker(1⊗i)$
    * $u = (κ⊗1)(u')$ where $κ : N → M$ is the inclusion.
* If $R$ is a domain, and $A$ is a flat $R$-module, then $A$ is torsion-free.
* Modules over PID are flat iff they are torsion-free.

 Tensor products may not commute with direct products:
 $$ ℚ ⊗_ℤ \prod_{n ≥ 2} ℤₙ \not≌ \prod_{n≥2} (ℚ ⊗_ℤ ℤₙ) $$

# Character Modules

$$ B^* = \Hom_ℤ(B, ℚ/ℤ) $$

## $A \overset{α}{→} B \overset{β}{→} C ⟺ C^* \overset{β^*}{→} B^* \overset{α^*}{→} A^*$

$⟹ \Hom_ℤ(-, ℚ/ℤ)$ is exact because $ℚ/ℤ$ is an injective $ℤ$-module.

$\impliedby$

$\im α ⊆ \ker β$. Let $αx ∈ \im α - \ker β$, then since $αx ∉ \ker β$ so
$βαx ≠ 0$.

*Exercise 3.19 (i): if $G$ is an abelian group and $a ∈ G$ is nonzero,
there is a homomorphism $f : G → ℝ/ℤ$ with $f(a) ≠ 0$.*

Treating $C$ as a $ℤ$-module, then there is an $f : C → ℚ/ℤ ∈ \Hom_ℚ(C, ℚ/ℤ)$
such that $fβα(x) ≠ 0$. Thus $f ∈ C^*$ and $fβα ≠ 0 ⟹ βα = α^*β^* ≠ 0$.
But this contradicts the hypothesis.

$\ker β ⊆ \im α$.

