---
header-includes: |
    - \usepackage{mathtools}
    - \usepackage{amsmath}
---

# Ring Theory

* Let $R$ be an integral domain and $p âˆˆ R$.
  If $âŸ¨pâŸ©$ is maximal then $p$ is irreducible.
* $I$ is a maximal ideal $â‡” R/I$ is a field.
    * Let $a âˆˆ R - I$. Then $aR + I = R â‡’ 1 âˆˆ ab + I$ for some $b$.
      So $(a + I)(b + I) = 1 + I$, and every $a âˆ‰ I$ has an inverse.
* Let $R$ be an integral domain and $p âˆˆ R$.
  Then $âŸ¨pâŸ©$ is prime $â‡”$ $p$ is prime.
* Let $R$ be a ring. Then $I$ is prime $â‡”$ $R/I$ is an integral domain.
    * $(a + I)(b + I) = I â‡’ a \text{ or } b âˆˆ I$
* Maximal ideals are prime.
* Finite integral domains are fields.

# Prime Ideals

## $â„¤_K/ğ”­$ is finite (lemma 5.20)

Let $ğ”­$ be a non-zero prime ideal in $â„¤_K$. Let $Î± âˆˆ ğ”­, Î± â‰  0$.
Then $N(Î±) âˆˆ â„¤$ and $Î± | N(Î±) â‡’ N(Î±) âˆˆ ğ”­$.

$â„¤_K$ has integral basis
$$â„¤_K = â„¤Ï‰_1 + â‹¯ + â„¤Ï‰_n$$
Since $NÏ‰_i âˆˆ ğ”­$ by the nature of ideals, then $a_i Ï‰_i â‰¡ b_i Ï‰_i \mod ğ”­$
where $0 â‰¤ b_i < N$. It could be smaller but we have established an upper
bound for $b_i$, so $â„¤_K/ğ”­$ is finite.

## $K$ is a number field. Every non-zero prime ideal $ğ”­ âŠ† â„¤_K$ is maximal (proposition 5.21)

Proof:

* Prime ideal $ğ”­ â‡’ â„¤_K/ğ”­$ is an integral domain.
* $â„¤_K/ğ”­$ is finite (lemma 5.20).
* Finite integral domain is a field.
* $â„¤_K/ğ”­$ is a field $â‡’ ğ”­$ is a maximal ideal.

# Fractional Ideals

## There are prime ideals $ğ”­_1, â€¦, ğ”­_r$ such that $ğ”­_1 â‹¯ ğ”­_r âŠ† ğ”$ (lemma 5.24)

$ğ”$ is a non-zero ideal of $â„¤_K$.

$â„¤_K$ is Noetherian.
Since $ğ”$ forms an ascending chain
$ğ” âŠ† ğ”_1 âŠ† ğ”_2 âŠ† â‹¯$,
it eventually terminates.

There are no prime ideals $ğ”­_1 â‹¯ ğ”­_r âŠ† ğ”$.
The same is true for all ideals in the chain $ğ”_i$.

Lets take $ğ”$ to be the largest ideal in the chain.

$ğ”$ is not prime otherwise $ğ”­_1 = ğ” âŠ† ğ”$
and the proof is finished.

So there are ideals $ğ”_1, ğ”_2$ in $â„¤_K$ such that
$ğ”_1 ğ”_2 âŠ† ğ”,
ğ”_1 âˆ‰ ğ”,
ğ”_2 âˆ‰ ğ”$
Write
$$ğ”Ÿ_1 = ğ” + ğ”_1,
ğ”Ÿ_2 = ğ” + ğ”_2$$
Then we can see that
$$ğ”Ÿ_1 ğ”Ÿ_2 = (ğ” + ğ”_1)(ğ” + ğ”_2)
= ğ” + ğ”_1 ğ” + ğ”_2 ğ” + ğ”_1 ğ”_2$$
Since $ğ”_1 ğ”_2 âŠ† ğ”$, so
$ğ”Ÿ_1 ğ”Ÿ_2 âŠ† ğ”$.
But also observe that
$$ğ” âŠŠ ğ”Ÿ_1, ğ” âŠŠ ğ”Ÿ_2$$

Since $ğ”Ÿ_1, ğ”Ÿ_2$ are bigger than $ğ”$, then by $ğ”$'s maximality,
there exist prime ideals $ğ”­_i$ such that
$$ğ”­_1 â‹¯ ğ”­_s âŠ† ğ”Ÿ_1$$
$$ğ”­_{s+1} â‹¯ ğ”­_t âŠ† ğ”Ÿ_2$$
$$â‡’ ğ”­_1 â‹¯ ğ”­_t âŠ† ğ”Ÿ_1 ğ”Ÿ_2
âŠ† ğ”$$
Which is a contradiction.

## $\mathfrak{a âŠ† b â‡’ b^{-1} âŠ† a^{-1}}$

Let $Î² âˆˆ ğ”Ÿ^{-1}$
$$Î² ğ”Ÿ âŠ† â„¤_K$$
but $ğ” âŠ† ğ”Ÿ â‡’ Î² ğ” âŠ† â„¤_K$ and so
$$Î² âˆˆ ğ”^{-1}$$

## $ğ”^{-1} = \{ Î± âˆˆ K : Î± ğ” âŠ† â„¤_K \}$ is a fractional ideal (lemma 5.25)

$$ğ”^{-1} = \{ Î± âˆˆ K : Î± ğ” âŠ† â„¤_K \}$$
Let $Î³ âˆˆ ğ”$ and $ğ”  = Î³ ğ”^{-1}$.
Take $i, i' âˆˆ ğ” $, then $i = Î³ Î², i' = Î³ Î²'$ with
$Î², Î²' âˆˆ ğ”^{-1}$.
$$(Î² + Î²') ğ” = Î² ğ” + Î²' ğ” âŠ† (â„¤_K + â„¤_K) = â„¤_K$$

Let $i = Î³ Î² âˆˆ ğ” $ with $Î³ âˆˆ ğ”, Î² âˆˆ ğ”^{-1}$ and $r âˆˆ â„¤_K$.
We want to show that $ri âˆˆ ğ” $.

But note that $r âˆˆ ğ”^{-1}$, so $r Î² âˆˆ ğ”^{-1} â‡’ ri = Î³ (r Î²) âˆˆ ğ” $.

```python
sage: K.<a> = NumberField(x^2 + 5)
sage: O = K.ring_of_integers()
sage: I = O.ideal(1 + a)
sage: (1 - a) * I
Fractional ideal (6)
sage: (1 - a)/6 * I
Fractional ideal (1)
sage: 1 - a in I^-1
True
sage: a in I^-1
True
sage: I.basis()
[6, a + 1]
sage: factor(I)
(Fractional ideal (2, a + 1)) * (Fractional ideal (3, a + 1))
```

## $ğ”$ is a proper ideal of $â„¤_K â‡’ â„¤_K âŠŠ ğ”^{-1}$ (lemma 5.26)

### $ğ” âŠ† ğ”Ÿ â‡’ ğ”Ÿ^{-1} âŠ† ğ”^{-1}$

Let $Î² âˆˆ ğ”Ÿ^{-1}$, then $Î² ğ”Ÿ âŠ† â„¤_K$.

But $ğ” âŠ† ğ”Ÿ â‡’ Î² ğ” âŠ† â„¤_K$

So $Î² âˆˆ ğ”^{-1}$.

Section 4.6 shows $âŸ¨1 - \sqrt{-5}âŸ©$ is not prime.

```python
sage: K.<a> = NumberField(x^2 + 5)
sage: O = K.ring_of_integers()
sage: I = O.ideal(1 + a)
sage: (1 - a) * I
Fractional ideal (6)
sage: (1 - a)/6 * I
Fractional ideal (1)
sage: 1 - a in I^-1
True
sage: a in I^-1
True
sage: I.basis()
[6, a + 1]
sage: I.is_prime()
False
sage: I.is_maximal()
False
sage: I
Fractional ideal (a + 1)
sage: factor(I)
(Fractional ideal (2, a + 1)) * (Fractional ideal (3, a + 1))
sage: J = O.ideal(2, a + 1)
sage: J.is_prime()
True
sage: 7 + a in J
True
sage: Î± = O.ideal(7 + a)
sage: factor(Î±)
(Fractional ideal (2, a + 1)) * (Fractional ideal (3, a + 1))^3
sage: J.is_prime(), J.is_maximal()  # of course
(True, True)
sage: O.ideal(3 + a+ 1)^3
Fractional ideal (43*a + 4)
sage: Î² = (43*a + 4)*(10 + a) # choose any random value from the ideal
sage: Î² in O.ideal(3 + a+ 1)^3
True
sage: Î² in Î±
False
sage: Î²*J
Fractional ideal (277830, 7*a + 150115)
sage: Î±
Fractional ideal (a + 7)
sage: 277830 in Î±
True
sage: 7*a + 150115 in Î±
True
sage: Î²*Î±^-1*J
Fractional ideal (5145, 7*a + 910)
sage: # which is a subset of Z_K
sage: Î²*Î±^-1
Fractional ideal (119/2*a + 35/2)
sage: J
Fractional ideal (2, a + 1)
sage: (119/2*a + 35/2)*J
Fractional ideal (5145, 7*a + 910)
sage: # so therefore Î²*Î±^-1 is a subset of J^-1
sage: J^-1
Fractional ideal (1, 1/2*a + 1/2)
sage: # we can see it consists of all odd halfs of a
sage: # and any integer multiple of 1/2
sage: # which Î²*Î±^-1 = <119/2*a + 35/2> is a member of
sage: (a + 7)*O
Fractional ideal (a + 7)
sage: Î²
434*a - 175
sage: N.<a> = Integers(5)[]
sage: N(a + 7)
a + 2
sage: N(434*a - 175)
4*a
sage: # so they are different
```

$$Î± âˆˆ ğ”­ â‡’ âŸ¨Î±âŸ©âŠ† ğ”­$$
And there exists 
$$ğ”­_1 â‹¯ ğ”­_r âŠ† âŸ¨Î±âŸ©$$
but since $r$ is minimal
$$ğ”­_2 â‹¯ ğ”­_r âŠˆ âŸ¨Î±âŸ©$$
Let $Î² âˆˆ ğ”­_2 â‹¯ ğ”­_r$, then $Î² âˆ‰ âŸ¨Î±âŸ©$.
$$Î²ğ”­ âŠ† ğ”­_1 â‹¯ ğ”­_r \implies Î²ğ”­ âŠ† âŸ¨Î±âŸ©$$
$$Î±^{-1} Î²ğ”­ âŠ† â„¤_K$$
$$Î±^{-1} Î² âˆˆ ğ”­^{-1}$$
But also $Î² âˆ‰ âŸ¨Î±âŸ©$
$$â‡’ Î±^{-1} Î² âˆ‰ â„¤_K$$

## $ğ”­$ is maximal $â‡’ ğ”­ğ”­^{-1} = â„¤_K$ (lemma 5.28)

$ğ”­^{-1}$ strictly contains $â„¤_K$, so there is a non-integer element $Î¸ âˆˆ ğ”­^{-1}$,
and $ğ”­Î¸ âŠˆ ğ”­$. But $ğ”­$ is maximal, so $ğ”­ğ”­^{-1} = â„¤_K$.

## $ğ”$ is any ideal $â‡’ ğ”ğ”^{-1} = â„¤_K$ (lemma 5.29)

By the prev lemma, max ideals $ğ”­ğ”­^{-1} = â„¤_K$. So $ğ”$ is not maximal.

### Derive identity

$ğ”ğ”­^{-1}$ is an ideal.
$$ğ” âŠ† ğ”ğ”­^{-1}$$
but $âˆƒÎ¸ âˆˆ ğ”­^{-1} : Î¸ âˆ‰ â„¤_K$ so $ğ” âŠŠ ğ”ğ”­^{-1}$.

Since $ğ”ğ”­^{-1}$ is an ideal, and $ğ”$ is the biggest such that
$ğ”ğ”^{-1} = â„¤_K$ then
$$ğ”ğ”­^{-1}(ğ”ğ”­^{-1}) = â„¤_K$$

### Prove final statement

$$ğ”ğ”­^{-1}(ğ”ğ”­^{-1}) = â„¤_K$$
$$[ğ”­^{-1}(ğ”ğ”­^{-1})] Â· ğ” = â„¤_K$$
$$ â‡’ ğ”­^{-1}(ğ”ğ”­^{-1}) âŠ† ğ”^{-1}$$
by the definition of a fractional ideal.
$$ â‡’ ğ”ğ”­^{-1}(ğ”ğ”­^{-1}) âŠ† ğ”ğ”^{-1}$$

## Every ideal $ğ” â‰  0$ is a product of prime ideals (lemma 5.31)

Every maximal ideal is prime.

Let $ğ”$ be the biggest ideal not a product of primes.
Then it is contained in $ğ”­$ prime and so we can write.
$$   ğ” ğ”­^{-1} =   ğ”­_1 â‹¯ ğ”­_r $$
$$ â‡’ ğ”        = ğ”­ ğ”­_1 â‹¯ ğ”­_r $$

# Norms of Ideals

## $N_{K/â„š}(âŸ¨Î±âŸ©) = |N_{K/â„š}(Î±)|$ (lemma 5.35)

### Index calculated from determinant

See Alaca ANT theorem 9.1.2.

Let $G$ be a free Abelian group with $n$ generators $Ï‰_1, â€¦, Ï‰_n$.
$$ G = \{ x_1 Ï‰_1 + â‹¯ + x_n Ï‰_n : x_i âˆˆ â„¤ \} $$
Let $H$ be a subgroup of $G$ generated by $n$ elements $Î·_1, â€¦, Î·_n$
$$ H = \{ y_1 Î·_1 + â‹¯ + y_n Î·_n : y_i âˆˆ â„¤ \} $$
Because each $Î·_i âˆˆ H âŠ† G$ we have
$$ Î·_i = c_{i, 1} Ï‰_1 + â‹¯ + c_{i, n} Ï‰_n $$
Let $C = (c_{i,j})$ be an $n Ã— n$ matrix. Then
$$ [G : H] = \begin{cases}
    |\det(C)| & \text{ if } \det(C) â‰  0 \\
    âˆ         & \text{ if } \det(C) = 0
\end{cases} $$
where $|\det(C)|$ means absolute value of C's determinant.

### Elements of ideal for $âŸ¨Î±âŸ©$

$$ âŸ¨Î±âŸ© = â„¤Î±Ï‰_1 + â‹¯ + â„¤Î±Ï‰_n $$

\begin{align*}
Î± Ï‰_1 &= a_{1,1} + â‹¯ + a_{n, 1} Ï‰_n \\
Î± Ï‰_2 &= a_{1,2} + â‹¯ + a_{n, 2} Ï‰_n \\
      & â‹¯ \\
Î± Ï‰_n &= a_{1,n} + â‹¯ + a_{n, n} Ï‰_n \\
\end{align*}

$$ Î±
\begin{pmatrix}
Ï‰_1 \\
\vdots \\
Ï‰_n
\end{pmatrix}
=
\begin{pmatrix}
a_{1,1} & \hdots & a_{n,1} \\
        & \hdots &         \\
a_{1,n} & \hdots & a_{n,n} \\
\end{pmatrix}
\begin{pmatrix}
Ï‰_1 \\
\vdots \\
Ï‰_n
\end{pmatrix}
$$
The definition of norm from 3.2, is given as the determinant of
that transform matrix.

# $N(ğ”ğ”Ÿ) = N(ğ”) N(ğ”Ÿ)$ (theorem 5.37)

Let $ğ”­$ be a non-zero prime ideal of $â„¤_K$.

## $â„¤_K / ğ”­ â‰… ğ” / ğ”ğ”­$ (lemma 5.36)

There is no ideal $ğ”Ÿ$ between $ğ”ğ”­ âŠŠ ğ”Ÿ âŠŠ ğ”$.
To see this simply multiply through by $ğ”^{-1}$, and note $ğ”­$ is maximal.
So either $ğ”Ÿ = ğ”$ or $ğ”ğ”­$.

Choose $Î± âˆˆ ğ”$ with $Î± âˆ‰ ğ”ğ”­$. Then because of above $âŸ¨Î±, ğ”ğ”­âŸ© = ğ”$.
$$ Ï• : â„¤_K â†’ ğ”/ğ”ğ”­ $$
$$ Ï•(x) = Î±x + ğ”ğ”­ $$
is surjective. The kernel is $âŸ¨ğ”­âŸ©$ since $Î±âŸ¨ğ”­âŸ© = ğ”ğ”­$.

The book has a typo on the last line of the proof.
It should be $â„¤_K / ğ”­ â‰… ğ” / ğ”ğ”­$.

## Result

Factorise $ğ”Ÿ$ into prime ideals and so we just deal with $ğ”Ÿ = ğ”­$.

$$ Ï• : â„¤_K/ğ”ğ”­  â†’  â„¤_K/ğ”  $$
$$ Ï•(Î± + ğ”ğ”­)   = Î± + ğ”   $$
is a homomorphism. So
$$ \left| \frac{ â„¤_K/ğ”ğ”­ }{ ğ”/ğ”ğ”­ } \right| = \left| \frac{ â„¤_K/ğ”ğ”­ }{ â„¤_K/ğ”­ } \right| = | â„¤_K/ğ” | $$
$$ â‡’ N(ğ”ğ”Ÿ) = |â„¤_K/ğ”ğ”­| = |â„¤_K/ğ”|Â·|â„¤_K/ğ”­| = N(ğ”) N(ğ”Ÿ) $$

# Dimension, Ramification Index and Inertia Degree

$â„¤_K$ is $n = [K:â„š]$ dimension vector space. See section 3.4.
$$ |â„¤_K / âŸ¨pâŸ©| = p^n $$
By CRT $â„¤_K / âŸ¨pâŸ© â‰… â„¤_K / ğ”­_1^{e_1} Ã— â„¤_K / ğ”­_r^{e_r}$.
$$ |â„¤_K/ğ”­_i^{e_i}| = N(p_i)^{e_i} = [â„¤_K/ğ”­_i : ğ”½_p]^{e_i} = (p^{f_i})^{e_i} $$

$$ n = e_1 f_1 + â‹¯ + e_r f_r $$

```python
sage: # See chapter 3.6.1
sage: y = ( (sqrt(2) + sqrt(6))/2 )
sage: minpoly(y)
x^4 - 4*x^2 + 1
sage: K.<a> = NumberField(x^4 - 4*x^2 + 1)
sage: O = K.ring_of_integers()
sage: I = O.ideal(5)
sage: I
Fractional ideal (5)
sage: factor(I)
(Fractional ideal (a^3 - 5*a + 1)) * (Fractional ideal (a^3 - 5*a - 1))
sage: A, B = O.ideal(a^3 - 5*a + 1), O.ideal(a^3 - 5*a - 1)
sage: A*B
Fractional ideal (5)
sage: A.ramification_index(), B.ramification_index()
(1, 1)
sage: I.norm()
625
sage: A.norm(), B.norm()
(25, 25)
sage: A.norm() * B.norm()
625
sage: ( ( y^3 - 5*y + 1 )*( y^3 - 5*y - 1) ).expand()
5
```

## Find Change of Basis Matrix

The ideal $âŸ¨Î³^3 - 5Î³ + 1âŸ©$ consists of elements $a + bÎ³ + cÎ³^2 + dÎ³^3 âˆˆ â„¤_K$
multiplied by $Î³^3 - 5Î³ + 1$.

$$ â„¤_K = â„¤[Î³], \qquad Î³ = \frac{\sqrt{2} + \sqrt{6}}{2}, \qquad Î± = \sqrt{6} - 1 $$
$$ â„¤_K = â„¤ + â„¤Î³ + â„¤y^2 + â„¤y^3 $$
$$ âŸ¨Î±âŸ© = â„¤Î± + â„¤Î±Î³ + â„¤Î±Î³^2 + â„¤Î±Î³^3 $$
$$ \sqrt{2} = Î³^3 - 3Î³, \qquad \sqrt{3} = Î³^2 - 2 $$
$$ Î± = -Î³^3 + 5Î³ - 1 $$
Elements in $âŸ¨Î±âŸ©$ are of the form
$$ (a + bÎ³ + cÎ³^2 + dÎ³^3)(-Î³^3 + 5Î³ - 1) $$
$$ \textrm{minpoly}(Î³) = Î³^4 - 4Î³^2 + 1 $$
$$ \implies Î³^4 = 4Î³^2 - 1 $$

```python
sage: var("a b c d y")
(a, b, c, d, y)
sage: Y = (sqrt(2) + sqrt(6))/2
sage: y4 = 4*y^2 - 1
sage: (y4.subs({y: Y}) - Y^4).expand()
0
sage: e = ( (a + b*y + c*y^2 + d*y^3)*(-y^3 + 5*y - 1) ).expand(); e
-d*y^6 - c*y^5 - b*y^4 + 5*d*y^4 - a*y^3 + 5*c*y^3 - d*y^3 + 5*b*y^2 - c*y^2 + 5*a*y - b*y - a
sage: e = e.subs({y^4: y4}).expand(); e
-d*y^6 - c*y^5 - a*y^3 + 5*c*y^3 - d*y^3 + b*y^2 - c*y^2 + 20*d*y^2 + 5*a*y - b*y - a + b - 5*d
sage: e = e.subs({y^5: y*y4}).expand(); e
-d*y^6 - a*y^3 + c*y^3 - d*y^3 + b*y^2 - c*y^2 + 20*d*y^2 + 5*a*y - b*y + c*y - a + b - 5*d
sage: e = e.subs({y^6: y^2*y4}).expand(); e
-4*d*y^4 - a*y^3 + c*y^3 - d*y^3 + b*y^2 - c*y^2 + 21*d*y^2 + 5*a*y - b*y + c*y - a + b - 5*d
sage: e = e.subs({y^4: y4}).expand(); e
-a*y^3 + c*y^3 - d*y^3 + b*y^2 - c*y^2 + 5*d*y^2 + 5*a*y - b*y + c*y - a + b - d
sage: e.collect(y)
-(a - c + d)*y^3 + (b - c + 5*d)*y^2 + (5*a - b + c)*y - a + b - d
```

$$
\begin{pmatrix}
    - a + b - d \\
    5a - b + c \\
    b - c + 5d \\
    -a + c - d
\end{pmatrix}
=
\begin{pmatrix}
    -1 &  1 &  0 & -1 \\
     5 & -1 &  1 &  0 \\
     0 &  1 & -1 &  5 \\
    -1 &  0 &  1 & -1 \\
\end{pmatrix}
\begin{pmatrix}
    a \\
    b \\
    c \\
    d \\
\end{pmatrix}
$$

```python
sage: A = matrix([
....:     [-1, 1, 0, -1],
....:     [5, -1, 1, 0],
....:     [0, 1, -1, 5],
....:     [-1, 0, 1, -1]
....: ])
sage: A.determinant()
25
```

## Calculate Index From Basis Transformation Matrix

We can perform 2 operations on this change of basis matrix which keep it valid.
See Alaca 9.1.2.

Let $G = \{ x_1 Ï‰_1 + x_2 Ï‰_2 + x_3 Ï‰_3 + x_4 Ï‰_4 : x_i âˆˆ â„¤ \}$
with a subgroup $H$ defined by a basis
$$Î·_i = c_{i,1} Ï‰_1 + c_{i,2} Ï‰_2 + c_{i, 3} Ï‰_3 + c_{i, 4} Ï‰_4$$
We can add and subtract these basis from each other leaving the subgroup $H$ intact.
Observe that
$$\{ Î·_1, Î·_2, Î·_3, Î·_4 \} \textrm{ and } \{ Î·_1, Î·_2 + k Î·_3, Î·_3, Î·_4 \}$$
both generate the same group.

There is a slightly more difficult column operation.
We simplify notation below.
Assume we are swapping columns 2 and 3 of the 2nd row.

\begin{align*}
Î·_2 &= c_1 Ï‰_1 + c_2 Ï‰_2 + c_3 Ï‰_3 + c_4 Ï‰_4 \\
    &= (c_1 Ï‰_1 + c_4 Ï‰_4) + c_2 Ï‰_2 + c_3 Ï‰_3 \\
    &= (c_1 Ï‰_1 + c_4 Ï‰_4) + (c_2 + c_3) Ï‰_2 + c_3 (Ï‰_3 - Ï‰_2) \\
    &= c_1 Ï‰_1 + \bar{c}_2 Ï‰_2 + c_3 \bar{Ï‰}_3 + c_4 Ï‰_4
\end{align*}
where
$$ \bar{c}_2 = c_2 + c_3, \qquad \bar{Ï‰}_3 = Ï‰_3 - Ï‰_2 $$
Which will leave also $G$ unchanged. Now we end up with
$$ G = âŸ¨\bar{Ï‰}_1, \bar{Ï‰}_2, \bar{Ï‰}_3, \bar{Ï‰}_4âŸ© $$
$$ H = âŸ¨d_1 \bar{Ï‰}_1, d_2 \bar{Ï‰}_2, d_3 \bar{Ï‰}_3, d_4 \bar{Ï‰}_4âŸ© $$
See the script ch5-degree.sage where we use this method to compute the degree.

## Using Ring Isomorphisms

$$
Ïƒ_1 : \begin{cases}
        \sqrt{2} &\mapsto \sqrt{2} \\
        \sqrt{3} &\mapsto \sqrt{3} \\
        \sqrt{6} &\mapsto \sqrt{6} \\
      \end{cases}
\qquad
Ïƒ_2 : \begin{cases}
        \sqrt{2} &\mapsto -\sqrt{2} \\
        \sqrt{3} &\mapsto \sqrt{3} \\
        \sqrt{6} &\mapsto -\sqrt{6} \\
      \end{cases}
\qquad
Ïƒ_3 : \begin{cases}
        \sqrt{2} &\mapsto \sqrt{2} \\
        \sqrt{3} &\mapsto -\sqrt{3} \\
        \sqrt{6} &\mapsto -\sqrt{6} \\
      \end{cases}
\qquad
Ïƒ_4 : \begin{cases}
        \sqrt{2} &\mapsto -\sqrt{2} \\
        \sqrt{3} &\mapsto -\sqrt{3} \\
        \sqrt{6} &\mapsto \sqrt{6} \\
      \end{cases}
$$
\begin{align*}
N(\sqrt{6} - 1) &= Ïƒ_1(\sqrt{6} - 1) Ïƒ_2(\sqrt{6} - 1) Ïƒ_3(\sqrt{6} - 1) Ïƒ_4(\sqrt{6} - 1) \\
                &= (\sqrt{6} - 1) (-\sqrt{6} - 1) (-\sqrt{6} - 1) (\sqrt{6} - 1) \\
                &= 25
\end{align*}

```python
sage: R.<x> = PolynomialRing(ZZ, 1)
sage: I = Ideal([x^4 - 4*x^2 + 1, x^3 - 5*x + 1])
sage: I.groebner_basis()
[x^2 + 4*x + 1, 5]
```

Which isomorphic to $ğ”½_{5^2}$.

# Deconstructing Primes into Ideals (prop 5.42)

## Short Explanation

$$ â„¤_K / âŸ¨pâŸ© â‰… ğ”½_p[Î³] â‰… ğ”½_p[X] / âŸ¨\bar{g}(X)âŸ© $$
By CRT
$$ ğ”½_p[X] / âŸ¨\bar{g}(X)âŸ© â‰… ğ”½_p[X] / âŸ¨\bar{g}_1(X)^{e_1}âŸ© Ã— â‹¯ Ã— ğ”½_p[X] / âŸ¨\bar{g}_r(X)^{e_r}âŸ© $$
The map $â„¤_K â†’ ğ”½_p[X] / âŸ¨\bar{g}_1(X)^{e_1}âŸ© Ã— â‹¯ Ã— ğ”½_p[X] / âŸ¨\bar{g}_r(X)^{e_r}âŸ©$ has kernel
$$ âŸ¨p, g_1(Î³)^{e_1}âŸ© âˆ© â‹¯ âˆ© âŸ¨p, g_r(Î³)^{e_r}âŸ© $$
$ğ”­_i^{e_i} âŠ† âŸ¨p, g_i(Î³)^{e_i}âŸ©$ because
$$ ğ”­_i^{e_i} = âŸ¨p^{e_i}, p^{e_i - 1} g_i(Î³), â€¦ , p g_i(Î³)^{e_i - 1}, g_i(Î³)^{e_i}âŸ© $$
Finally
$$ âŸ¨pâŸ© = âŸ¨p, g_1(Î³)^{e_1}âŸ© âˆ© â‹¯ âˆ© âŸ¨p, g_r(Î³)^{e_r}âŸ© $$
$$ â‡’ ğ”­_1^{e_1} â‹¯ ğ”­_r^{e_r} âŠ† âŸ¨pâŸ© $$
Taking norms, we see that $n = e_1 f_1 + â‹¯ + e_r f_r$, so the inclusion is actually an equality.

## Example

$$ K = â„š(\sqrt{2}, \sqrt{3}) $$
$$ Î³ = \frac{ \sqrt{2} + \sqrt{6} }{ 2 } $$
$$ g(X) = X^4 - 4X^2 + 1 $$
$$ p = 5 $$
\begin{align*}
\bar{g}(X) &= X^4 + X^2 + 1 \\
           &= (X^2 + X + 1)(X^2 + 4X + 1)
\end{align*}
$$ g_1(X) = (X^2 + X + 1), g_2(X) = X^2 + 4X + 1 $$
$$ ğ”­_1 = âŸ¨5, Î³^2 + Î³ + 1âŸ©, ğ”­_2 = âŸ¨5, Î³^2 + 4Î³ + 1âŸ© $$

## Double Quotienting Ideals Isomorphic to Sum of Ideals

Observe the lattice when we collapse normal subgroups down to 0.

$$ \frac{ âŸ¨pâŸ© }{ âŸ¨g(X)âŸ© } âŠ† \frac{ â„¤[X] }{ âŸ¨g(X)âŸ© } â‡” âŸ¨pâŸ© âŠ† â„¤[X] $$

$$ Ï• : â„¤[X] / âŸ¨g(X)âŸ© â†’ â„¤[X] / âŸ¨p, g(X)âŸ© $$
$$ Ï•(r + âŸ¨g(X)âŸ©) = r + âŸ¨p, g(X)âŸ© $$
$$ \ker Ï• = âŸ¨p, g(X)âŸ© $$

Then observe
$$ Ï•(r + âŸ¨g(X)âŸ©) = 0 â‡” r âˆˆ âŸ¨p, g(X)âŸ© â‡” r + âŸ¨g(X)âŸ© âˆˆ âŸ¨p, g(X)âŸ© $$

By first iso theorem with the homomorphism $Ï•$, we see that
$$ (â„¤[X] / âŸ¨g(X)âŸ©) / âŸ¨p, g(X)âŸ© â‰Œ â„¤[X] / âŸ¨p, g(X)âŸ© $$

Alternatively we can observe that $âŸ¨g(X)âŸ© âŠ† âŸ¨p, g(X)âŸ© âŠ† â„¤[X]$, and then
by the third theorem
$$ \frac{ â„¤[X] / âŸ¨g(X)âŸ© }{ âŸ¨p, g(X)âŸ© / âŸ¨g(X)âŸ© } â‰Œ \frac{ â„¤[X] }{ âŸ¨p, g(X)âŸ© } $$
since $âŸ¨p, g(X)âŸ© / âŸ¨g(X)âŸ© = âŸ¨p, g(X)âŸ©$.

## $â„¤_K / ğ”­_1 â‰… ğ”½_p[X] / âŸ¨\bar{g}_1(X)âŸ©$ and is a Field

$$ â„¤_K / ğ”­_1 = â„¤[Î³] / âŸ¨5, Î³^2 + Î³ + 1âŸ© $$

$$ Ï• : â„¤[Î³] â†’ â„¤[X] / âŸ¨g(X)âŸ© $$
$$ Ï•(a_0 + a_1 Î³ + a_2 Î³^2 + a_3 Î³^3) = a_0 + a_1 X + a_2 X^2 + a_3 X^3 + âŸ¨g(X)âŸ© $$

$$ \frac{ â„¤[Î³] }{ âŸ¨p, g_1(Î³)âŸ© } â‰… \frac{ â„¤[X] / âŸ¨g(X)âŸ© }{ âŸ¨p, g_1(X), g(X)âŸ© / âŸ¨g(X)âŸ© } â‰… \frac{ â„¤[X] }{ âŸ¨p, g_1(X), g(X)âŸ© }$$

But also going in reverse with $Ïˆ : â„¤[X] / âŸ¨pâŸ© â†’ ğ”½_p$
$$ \frac{ â„¤[X] }{ âŸ¨p, g_1(X), g(X)âŸ© } â‰… \frac{ â„¤[X] / âŸ¨pâŸ© }{ âŸ¨p, g_1(X), g(X)âŸ© / âŸ¨pâŸ© } â‰… \frac{ ğ”½_p[X] }{ âŸ¨\bar{g}_1(X), \bar{g}(X)âŸ© } $$
Note that $\bar{g}_1(X) | \bar{g}(X)$
$$ â„¤_K / ğ”­_1 â‰… ğ”½_p[X] / âŸ¨\bar{g}_1(X)âŸ© $$

$\bar{g}_1(X)$ is irreducible $â‡’ âŸ¨\bar{g}_1(X)âŸ©$ is a prime ideal $â‡’$ the right hand side is a field,
and so $ğ”­_1$ is a prime ideal.

## $â„¤_K / âŸ¨pâŸ© â‰… ğ”½_p[X] / âŸ¨\bar{g}(X)âŸ©$

\begin{align*}
â„¤_K / âŸ¨pâŸ©   &= â„¤[Î³] / âŸ¨pâŸ© \\
            &â‰… \frac{ â„¤[X] / âŸ¨g(X)âŸ© }{ âŸ¨p, g(X)âŸ© / âŸ¨g(X)âŸ© } \\
            &= \frac{ â„¤[X] }{ âŸ¨p, g(X)âŸ© } \\
            &â‰… \frac{ â„¤[X] / âŸ¨pâŸ© }{ âŸ¨p, g(X)âŸ© / âŸ¨pâŸ© } \\
\end{align*}
But let $r âˆˆ âŸ¨p, g(X)âŸ© / âŸ¨pâŸ© âŠ† â„¤[X] / âŸ¨pâŸ©$, then $r = ap + bg(X) âˆˆ âŸ¨p, g(X)âŸ© + âŸ¨pâŸ© = âŸ¨p, g(X)âŸ©$

\begin{align*}
\frac{ â„¤[X] / âŸ¨pâŸ© }{ âŸ¨p, g(X)âŸ© / âŸ¨pâŸ© }
    &= \frac{ â„¤[X] / âŸ¨pâŸ© }{ âŸ¨p, g(X)âŸ© } \\
    &â‰… \frac{ ğ”½_p[X] }{ âŸ¨\bar{g}(X)âŸ© } \\
    &â‰… â„¤_K / âŸ¨pâŸ©
\end{align*}

## Deconstructing $pâ„¤_K$

There is a map $â„¤_K â†’ â„¤_K / âŸ¨pâŸ©$ with kernel $âŸ¨pâŸ©$.

Then for each component of the decomposed $â„¤_K / âŸ¨pâŸ©$, there is another map
$â„¤_K / âŸ¨pâŸ© â†’ â„¤_K / ğ”­_1 â‰… ğ”½_p[X] / âŸ¨\bar{g}_1(X)âŸ©$ by $Î³ â†’ X \mod âŸ¨p, g_1(X)âŸ©$.
So the kernel is $âŸ¨p, g_1(Î³)âŸ©$.
$$ pâ„¤_K = ğ”­_1^{e_1} â‹¯ ğ”­_r^{e_r} $$

