---
header-includes: |
    - \newcommand{\leg}[2]{\left( \frac{#1}{#2} \right)}
    - \newcommand{\âˆš}[1]{\sqrt{#1}}
---
# Polynomial $Î»_n(x)$ is irreducible

## Discriminant $Î” = Â±nâ¿$

Let $f_n(x) = xâ¿ - 1$ and the discriminant
$$ Î” = \prod_{i < j} (Î¶â± - Î¶Ê²)Â² $$
$$ f_n'(x) = (x - Î¶â‚‚)â‹¯(x - Î¶_n) + (x - Î¶â‚)(x - Î¶â‚ƒ)â‹¯(x - Î¶_n) + â‹¯ + (x - Î¶â‚)â‹¯(x - Î¶_{n - 1}) $$
$$ â‡’ f_n'(Î¶â‚) = (Î¶â‚ - Î¶â‚‚)â‹¯(Î¶â‚ - Î¶_n) $$

\begin{alignat*}{2}
n &= 1 \qquad Î” &&= 1 \\
n &= 2 \qquad Î” &&= (Î¶Â¹ - Î¶Â²)Â² \\
n &= 3 \qquad Î” &&= (Î¶Â¹ - Î¶Â²)Â² (Î¶Â¹ - Î¶Â³)Â² (Î¶Â² - Î¶Â³)Â² \\
n &= 4 \qquad Î” &&= (Î¶Â¹ - Î¶Â²)Â² (Î¶Â¹ - Î¶Â³)Â² (Î¶Â² - Î¶Â³)Â² (Î¶Â¹ - Î¶â´)Â² (Î¶Â² - Î¶â´)Â² (Î¶Â³ - Î¶â´)Â²
\end{alignat*}

$$ Î” = \prod_{i â‰  j} (Î¶â± - Î¶Ê²)Â² $$

$$ \prod_{i < j} (Î¶â± - Î¶Ê²)Â² = \prod_{j=1}^n f_n'(Î¶â±) $$

But $f_n'(x) = nx^{n - 1}$
$$ Î” = nâ¿ \left( \prod_{j = 1}^n Î¶â± \right)^{n - 1} $$
If $n â‰¡ 0 \mod{2}$ then $\frac{nÂ²}{2} + \frac{n}{2} â‰¡ b \mod{n}$ for some $b âˆˆ â„¤$
where $b = \frac{n}{2}$ so in this case $\sum_{i = 1}^n i â‰¡ n/2 \mod{n}$.
Otherwise it is 0.

```python
>>> for i in range(1, 10):
...     print(i, (sum(x for x in range(i+1)) % i) / i)
... 
1 0.0
2 0.5
3 0.0
4 0.5
5 0.0
6 0.5
7 0.0
8 0.5
9 0.0
```
So we see
$$ \prod_{j = 1}^n Î¶â± = Â±1 $$
$$ Î” = Â±nâ¿ $$

## $g(x)$ divides $f_n(x)$ and contains one primitive root means it has all roots

*Let there be a $g(x) âˆˆ â„¤[x]$ such that $g(x)|f_n(x)$ with $g(Î¶) = 0$.
We claim $g(Î¶áµ–) = 0$ for all prime $p âˆ¤ n$.*

Suppose $g(Î¶áµ–) â‰  0$. Since $f_n(x) = (x - Î¶â‚)â‹¯(x - Î¶_n)$ and $g|f_n$, so
for some $d$
$$ g(x) = (x - Î¶â‚)â‹¯(x - Î¶_d) $$
Then $g(Î¶áµ–)$ is the product of differences for nth roots of unity, hence
it divides the discriminant $Â±nâ¿$.

Let $Î¦_p$ be the Frobenius automorphism in mod $p$ and note
$$ Î¦_p(g(x)) â‰¡ g(Î¦_p(x)) \mod{p} $$
$$ â‡’ p | g(Î¶áµ–) - g(Î¶)áµ– $$
but $g(Î¶) = 0$ so $p | g(Î¶áµ–)$.

$$ p | g(Î¶áµ–), \quad g(Î¶áµ–) | nâ¿ â‡’ p | nâ¿ â‡’ p | n $$
which is a contradiction. So we get the result.

## $g(x)$ is $Î»_n(x)$

Let $g(x)$ be a nontrivial factor of $Î»_n(x)$ and therefore of $f_n(x)$.

As before let $Î¶$ be a primitive nth root of unity with $g(Î¶) = 0$.

Then for all primes $p âˆ¤ n$ the previous result states $g(Î¶áµ–) = 0$.

$$ Î¼ = \{ Î¶áµ : \gcd(k, n) = 1 \} $$
are all the primitive roots for $n$. So it follows $Î¶áµ$ for any $k$ coprime to $n$
is also a primitive $n$th root of unity.

Let $k$ be comprime to $n$. Write $k = pâ‚ â‹¯ p_m$.

Then $g(Î¶^{pâ‚}) = 0$ and $Î¶^{pâ‚}$ is a primitive root.

Now let $q_{i + 1} = q_i p_{i + 1}$ with $q_i = pâ‚$. By the same argument,
$g(Î¶^{q_{i + 1}}) = 0$.

Since $k = q_{i + 1}$, we see $g(Î¶áµ) = 0$ so every primitive $n$th root of unity
is a root of $g(x) â‡’ g(x) = Î»_n(x)$.

$g(x)$ is a generic polynomial dividing $f_n(x)$, so this argument means $Î»_n(x)$
is irreducible, since $g(x)$ must $Î»_n(x)$ and there are no smaller divisors.

# Exercises

## 9.2

\begin{align*}
Î¶Â²â¿ &= 1 \\
    &= (Î¶â¿)Â²
\end{align*}
so $Î¶â¿ = Â±1$, but $Î¶$ is a primitive $2n$ root of unity so $Î¶â¿ = -1$.

$n$ is odd, so $(-1)â¿ = -1$
$$ â‡’ -Î¶â¿ = 1 \textrm{ or } (-Î¶)â¿ = 1 $$
so $-Î¶$ is a primitive $n$th root of unity.

## 9.3.1

$$ m | n â‡’ m = pâ‚^{kâ‚} â‹¯ p_r^{k_r}, \; n = m pâ‚^{lâ‚} â‹¯ p_r^{l_r} qâ‚^{mâ‚} â‹¯ q_t^{m_t} $$
$$ mn = mÂ² pâ‚^{lâ‚} â‹¯ p_r^{l_r} n $$
$$ \gcd(mÂ² pâ‚^{lâ‚} â‹¯ p_r^{l_r}, nâ‚) = 1 $$
$$ â‡’ ğœ™(mn) = ğœ™(mÂ² pâ‚^{lâ‚} â‹¯ p_r^{l_r}) ğœ™(nâ‚) $$
\begin{align*}
ğœ™(p^{2k + l}) &= p^{2k + l} - p^{2k + l - 1} \\
    &= p^k (p^{k + l} - p^{k + l - 1})
\end{align*}
$$ ğœ™(mÂ² pâ‚^{lâ‚} â‹¯ p_r^{l_r}) = m ğœ™(m pâ‚^{lâ‚} â‹¯ p_r^{l_r}) $$
and so we see
$$ \deg Î»_{mn}(x) = \deg Î»_n(x^m) $$

## 9.3.2

Let $y : Î»_n(y) = 0$, then $y â‰  1$.
For any $a : Î»_n(aáµ) = 0 â‡’ aáµ â‰  0$, so $a$ is a primitive root of $Î»_{mn}(x)$.

We can divide each poly by $(x - a)$ and since they have the same degree,
we see $Î»_{mn}(x) = Î»_n(xáµ)$.

## 9.3.3

Let $g(x) = x^{p^{1 - r}}$, then we can compose the functions
$$ (Î»_p âˆ˜ g)(x^{p^{r - 1}}) = Î»_p(x) $$
$$ (Î»_{pÊ³} âˆ˜ g)(x) = Î»_{pÊ³}(x^{p^{1 - r}}) $$
So observe $pÊ³ = p^{1 - r} p^{2r - 1} â‡’ p^{1 - r} | pÊ³$.

Let $mn = p$ so that $m = p^{1 - r}, n = pÊ³$ then
$$ Î»_p(x) = Î»_{p^r}(x^{p^{1 - r}}) $$
now compose with $gâ»Â¹$ to get
$$ Î»_{pÊ³}(x) = Î»_p(x^{p^{r - 1}}) $$

### 9.4

$$ Î»_p(x) = \frac{xáµ– - 1}{x - 1} $$
$$ Î»â‚(x) = x - 1 $$
$$ xâ¿ - 1 = Î»â‚(x) Î»_p(x) Î»_q(x) Î»_{pq}(x) $$
Rearrange this last identity and we get
\begin{align*}
Î»_q(x) Î»_{pq}(x) &= \frac{ xâ¿ - 1 }{ Î»â‚(x) Î»_p(x) } \\
    &= \frac{ (xáµ–)^q - 1 }{ (x - 1) Â· \frac{ xáµ– - 1 }{ x - 1} } \\
    &= Î»_q(xáµ–)
\end{align*}


# Discriminants and Integral Bases

## $pâ„¤_K = âŸ¨1 - Î¶âŸ©^{ğœ™(pÊ³)}$

We can see
$$ Î»_{pÊ³}(X) = X^{p^{r - 1} (p - 1)} + X^{p^{r - 1} (p - 2)} + â‹¯ + X^{p^{r - 1}} + 1 \tag{1}$$
Just multiply the denominator out and you can see this holds.

Then the primitive roots are $Î¶áµ$ with $g âˆˆ G = \{ 1 â‰¤ g â‰¤ n | \gcd(p, g) = 1 \}$. You can
see that that any $g^{pâ±}$ is not primitive hence we exclude those.

$$ Î»_{pÊ³}(X) = \prod_{g âˆˆ G} (X - Î¶áµ) \tag{2}$$

Put $X = 1$ into (1), and we get $Î»_{pÊ³}(1) = p$ since there are $p - 1$ terms $+ 1$.
Then also substituting into (2) shows

$$ p = \prod_{g âˆˆ G} (1 - Î¶áµ) $$
$$ â‡’ âŸ¨pâŸ© = \prod_{g âˆˆ G} âŸ¨1 - Î¶áµâŸ© $$

$$ 1 - Î¶áµ = (1 - Î¶)(1 + Î¶ + â‹¯ + Î¶^{g - 1}) $$
which shows $âŸ¨1 - Î¶áµâŸ© âŠ† âŸ¨1 - Î¶âŸ©$.
And we can calculate the converse by finding $h : gh â‰¡ 1 \mod{pÊ³}$ since $Î¶^{gh} = Î¶Â¹$.
So both ideals are the same.

Lastly $[â„š(Î¶) : â„š] = ğœ™(pÊ³)$. To see this write $â„š(Î¶)$ in terms of its basis over $â„š$.
Then you see the generators are all the primitive elements which is $ğœ™(pÊ³)$.

## Ring of Integers $â„¤_K = â„¤[Î¶]$

$$ Î”\{Ï‰â‚, â€¦, Ï‰_n \} â„¤_K âŠ† â„¤Ï‰â‚ + â‹¯ + â„¤Ï‰_n $$
$$ Î”\{1, Î¶, â€¦, Î¶^{k - 1}\} = Â±pË¢ $$
$$ pË¢ â„¤_K âŠ† â„¤[Î¶] = â„¤ + â„¤Î¶ + â‹¯ + â„¤Î¶^{k - 1} âŠ† â„¤_K $$

From section 5, we know $pâ„¤_K = âŸ¨Ï€âŸ©áµ â‡’ k = [â„š(Î¶) : â„š]$.

### $â„¤_K = â„¤ + Ï€â„¤_K$

We know $N_{â„š(Î¶)/â„š}(Ï€) = p$. By definition $N_{â„š(Î¶)/â„š}(Ï€) = |â„¤_K / âŸ¨Ï€âŸ©|$ which we see is $p$,
so $|â„¤_K/âŸ¨Ï€âŸ©| = p$. Now lets consider the cosets
$$ a + âŸ¨Ï€âŸ©, \quad a âˆˆ â„¤ $$
Now we show correspondence of cosets mod $p$.

Take $a, a' âˆˆ â„¤$ with $a â‰¡ a' \mod{p}$, then since $âŸ¨pâŸ© âŠ‚ âŸ¨Ï€âŸ©$ we have $a â‰¡ a' \mod{âŸ¨Ï€âŸ©}$.

Likewise let $a â‰¡ a' \mod{âŸ¨Ï€âŸ©}$, then $a - a' âˆˆ âŸ¨Ï€âŸ© â‡’ âŸ¨a - a'âŸ© âŠ† âŸ¨Ï€âŸ©$, and so
$âŸ¨a - a'âŸ© = âŸ¨Ï€âŸ©Q$ for some ideal of $â„¤_K$.

Note that $N(a - a') = (a - a')Â²$ and $N(a - a') = N_{â„š(Î¶)/â„š}(âŸ¨a - a'âŸ©)$ so
\begin{align*}
(a - a') &= N_{â„š(Î¶)/â„š}(âŸ¨a - a'âŸ©) \\
    &= N_{â„š(Î¶)/â„š}(âŸ¨Ï€âŸ©Q) \\
    &= N_{â„š(Î¶)/â„š}(âŸ¨Ï€âŸ©) N_{â„š(Î¶)/â„š}(Q) \\
    &= p N_{â„š(Î¶)/â„š}(Q) \\
\end{align*}
so we see $p | (a - a')Â²$ and since $p$ is prime $p | (a - a')$ and $a â‰¡ a' \mod{p}$ so
$$ a â‰¡ a' \mod{âŸ¨Ï€âŸ©} â‡” a â‰¡ a' \mod{p} $$
so we see the cosets $a + âŸ¨Ï€âŸ© : a âˆˆ \{ 0, â€¦, p - 1 \}$ are distinct and
$$ â„¤_K / âŸ¨Ï€âŸ© â‰… â„¤ / âŸ¨pâŸ© $$

Since the cosets of $â„¤_K$ are $a + âŸ¨Ï€âŸ©, a âˆˆ â„¤$, we see $â„¤_K = â„¤ + Ï€â„¤_K$.

# Gauss Sums and Quadratic Reciprocity


$$ Ï„ = \leg{1}{23}Î¶ + â‹¯ + \leg{22}{23}Î¶Â²Â² $$
$$ Ï„Â² = \leg{1}{23}Î¶ \left[\leg{1}{23}Î¶ + â‹¯ + \leg{22}{23}Î¶Â²Â²\right] â‹¯ + \leg{22}{23}Î¶Â²Â² \left[\leg{1}{23}Î¶ + â‹¯ + \leg{22}{23}Î¶Â²Â²\right] $$
Let $c = aâ»Â¹ b \mod{23} â‡’ b = ac \mod{23}$ and then follow the steps.

$$ 1 + Î¶ + â‹¯ + Î¶Â²Â² = 0 â‡’ \sum_{a = 0}^{22} Î¶áµáµƒ = 0 $$
so we see $\sum_{a = 1}^{23} Î¶áµáµƒ = -1$.

Lastly also note $22 â‰¡ -1 \mod{23} â‡’ \leg{22}{23} = \leg{-1}{23} = -1$.

## Exercise 9.6: Generalize Above to $p$ Prime

$$ Ï„ = \leg{1}{p} Î¶ + â‹¯ + \leg{p - 1}{p} Î¶áµ–â»Â¹ $$
$$ Ï„Â² = \leg{1}{p} Î¶ \left[ \leg{1}{p} Î¶ + â‹¯ + \leg{p - 1}{p} Î¶áµ–â»Â¹ \right] + â‹¯ + \left[ \leg{1}{p} Î¶ + â‹¯ + \leg{p - 1}{p} Î¶áµ–â»Â¹ \right] $$
$$ b = ac \mod{p} $$
\begin{align*}
Ï„Â² &= \sum_{a = 1}^{p - 1} \sum_{c = 1}^{p - 1} \leg{aÂ²c}{p} Î¶áµƒâºáµƒá¶œ \\
    &= \sum_{a = 1}^{p - 1} \sum_{c = 1}^{p - 2} \leg{aÂ²c}{p} Î¶áµƒâ½Â¹âºá¶œâ¾ + \sum_{a = 1}^{p - 1} \leg{aÂ²(p - 1)}{p} Î¶áµƒâ½Â¹âºâ½áµ–â»Â¹â¾â¾ \\
    &= \sum_{a = 1}^{p - 1} \sum_{c = 1}^{p - 2} \leg{c}{p}   Î¶áµƒâ½Â¹âºá¶œâ¾ + \sum_{a = 1}^{p - 1} \leg{-1}{p} \\
\end{align*}
From Pinter chapter 23, H7 we know
$$ \leg{-1}{p} = \begin{cases}
1  \; \textrm{ if } p â‰¡ 1 \mod{4} \\
-1 \; \textrm{ if } p â‰¡ 3 \mod{4} \\
\end{cases} $$
$$ Ï„Â² = \sum_{c = 1}^{p - 2} \left[ \leg{c}{p} \sum_{a = 1}^{p - 1} Î¶áµƒâ½Â¹âºá¶œâ¾ \right] + (p - 1) \leg{-1}{p} $$
Since $Î¶$ is primitive and $Î¶â¿ - 1 = 0$, then since $\frac{Xâ¿ - 1}{X - 1} = 1 + â‹¯ + Xâ¿â»Â¹$, we can see $\sum_{a = 0}^{p - 1} Î¶áµƒ = 0$
or $1 + \sum_{a = 1}^{p - 1} Î¶áµƒ = 0 â‡’ \sum_{a = 1}^{p - 1} Î¶áµƒáµ = -1$ for $k â‰¢ 0 \mod{p - 1}$.

Set $k = 1 + c$ and we see
\begin{align*}
Ï„Â² &= \left[ \sum_{c = 1}^{p - 2} \leg{c}{p} Â· (-1) \right] + (p - 1) \leg{-1}{p} \\
   &= - \sum_{c = 1}^{p - 2} \leg{c}{p} + (p - 1) \leg{-1}{p} \\
\end{align*}
With $â„¤_p^* = \{ 1, â€¦, p - 1 \}$, we can create the group endomorphism $h : â„¤_p^* â†’ â„¤_p^*$ by $h(a) = aÂ²$.
The range of $h$ has $(p - 1)/2$ elements, which means we can split $â„¤_p^*$ into two cosets: quadratic residues and nonresidues.
We therefore see
\begin{align*}
\sum_{c = 1}^{p - 1} \leg{c}{p} &= \leg{1}{p} + â‹¯ + \leg{p - 1}{p} = 0\\
    &= \leg{1}{p} + â‹¯ + \leg{p - 2}{p} + \leg{-1}{p} \\
    &= \sum_{c = 1}^{p - 2} \leg{c}{p} + \leg{-1}{p}
\end{align*}
$$ â‡’ \sum_{c = 1}^{p - 2} \leg{c}{p} = - \leg{-1}{p} $$

\begin{align*}
Ï„Â² &= \leg{-1}{p} + (p - 1) \leg{-1}{p} \\
   &= \leg{-1}{p} p \\
\end{align*}

## Quadratic Reciprocity

Since $q$ is a prime distinct from $p$, both $1$ and $q$ generate the same set additively.
Therefore we conclude $\{ 1, â€¦, p - 1 \}$ and $\{ q, â€¦, (p - 1)q \}$ are the same sets.
You can also form the additive group homomorphism $h(a) = qa$ which has kernel $\{ 0 \}$, hence
is an isomorphism, and a permutation of the set.

So $â„¤_p^* = qâ„¤_p^*$, and $f(â„¤_p^*) = f(qâ„¤_p^*)$.
$$ \sum_{a = 1}^{p - 1} \leg{aq}{p} Î¶^{aq} = \sum_{a = 1}^{p - 1} \leg{a}{p} Î¶áµƒ $$
$$ â‡’ \leg{q}{p} Ï„(Î¶^q) = Ï„(Î¶) \tag{1} $$

We now show $Ï„(Î¶^q) â‰¡ Ï„(Î¶)^q \mod {q}$. First note that under the frobenius $Î¦(x + y) = Î¦(x) + Î¦(y)$.
Secondly $\leg{aÂ²}{p} = 1$, so for $q$ odd prime, $\leg{a}{p}^q = \leg{a}{p}$. Then we can apply this
\begin{align*}
Î¦(Ï„(Î¶)) &â‰¡ Î¦\left(\leg{1}{p}\right) Î¦(Î¶) + â‹¯ + Î¦\left(\leg{p - 1}{p}\right) Î¦(Î¶áµ–â»Â¹) \mod{q} \\
     &â‰¡ \leg{1}{p} Î¶^q + â‹¯ + \leg{p - 1}{p} Î¶áµ–â»Â¹ \mod{q} \\
     &â‰¡ Ï„(Î¦(Î¶))
\end{align*}
$$ â‡’ Ï„(Î¶^q) â‰¡ Ï„(Î¶)^q \mod{q} $$
Then from the previous exercise we saw that $Ï„(Î¶)Â² = \leg{-1}{p} p$
\begin{align*}
Ï„(Î¶)^q &= Ï„(Î¶) Ï„(Î¶)^{q - 1} \\
    &= Ï„(Î¶) \left(Ï„(Î¶)Â²\right)^{(q - 1)/2} \\
    &= Ï„(Î¶) p^{*(q - 1)/2} \\
    &â‰¡ Ï„(Î¶) \leg{p^*}{q} \mod{q} \qquad \textrm{(by Euler's criterion)}
\end{align*}
Substituting (1) into this, we get
$$ Ï„(Î¶^q) â‰¡ \leg{q}{p} Ï„(Î¶^q) \leg{p^*}{q} \mod{q} $$
Since the only values for legendre symbols are $\{ -1, 1 \}$ we conclude
$$ \leg{q}{p} \leg{p^*}{q} = 1 $$
$$ â‡’ \frac{1}{\leg{q}{p} \leg{p}{q}} = (-1)^{(p - 1)(q - 1)/4} $$
whereby the result easily follows.

# Ex 9.7

$$ Ï = \frac{1 + \âˆš{-23}}{2} $$
$$ â„š(\âˆš{-23}) $$
$$ ğ”­ = âŸ¨2, ÏâŸ© $$
$$ ğ”­Â³ = âŸ¨2Â³, 2Â²Ï, 2ÏÂ², ÏÂ³âŸ© $$
$$ \textrm{minpoly}(Ï) = XÂ² - X + 6 $$
$$ d â‰¡ 1 \mod{4} $$
\begin{align*}
â„¤_K &â‰… â„¤[X] / âŸ¨XÂ² - X + 6, 2, XâŸ© \\
    &â‰… â„¤[X] / âŸ¨2, XâŸ© \\
    &â‰… ğ”½â‚‚
\end{align*}
$$ N_{â„š(\âˆš{-23})/â„š}(ğ”­) = 2 $$
$$ (a + b\âˆš{-23})\left(\frac{3 - \âˆš{-23}}{2}\right) = \frac{3a + 23b}{2} + \frac{-a + 3b}{2} $$
$$ \begin{pmatrix}
3/2 & 23/2 \\
-1/2 & 3/2
\end{pmatrix}
\begin{pmatrix}
a \\ b
\end{pmatrix} =
\begin{pmatrix}
c \\ d
\end{pmatrix}
$$

```python
sage: var("x")
x
sage: K.<z> = NumberField(x^2 + 23)
sage: z^2
-23
sage: L.<a, b> = K[]
sage: (a + b*z)*(3 - z)/2
(-1/2*z + 3/2)*a + (3/2*z + 23/2)*b
sage: K.<a, b> = QQ[]
sage: L.<z> = K.extension(x^2 + 23)
sage: (a + b*z)*(3 - z)/2
(-1/2*a + 3/2*b)*z + 3/2*a + 23/2*b
sage: M = matrix([[3/2, 23/2], [-1/2, 3/2]])
sage: M.determinant()
8
sage: M^-1
[  3/16 -23/16]
[  1/16   3/16]
sage: M^-1 * vector([1/2, 1/2])
(-5/8, 1/8)
sage: M^-1 * vector([2, 0])
(3/8, 1/8)
sage: y = (3 - z)/2
sage: (-5 + z)*y/8
1/2*z + 1/2
sage: (3 + z)*y/8
2
```

So we see that
$$ \left(\frac{-5 + \âˆš{-23}}{8}\right) \left(\frac{3 - \âˆš{-23}}{2}\right) = Ï $$
$$ \left(\frac{3 + \âˆš{-23}}{8}\right) \left(\frac{3 - \âˆš{-23}}{2}\right) = 2 $$

$$ N\left(\frac{3 - \âˆš{-23}}{2}\right) = 8 $$
$$ N_{â„š(\âˆš{-23})/â„š}(ğ”­Â³) = 8 $$

# Ex 9.8

```python
sage: K.<z> = CyclotomicField(23)
sage: z^23
1
sage: (1 + z + z^5 + z^6 + z^7 + z^9 + z^11)*(1 + z^2 + z^4 + z^5 + z^6 + z^10 + z^11)
2*z^17 + 2*z^16 + 2*z^15 + 2*z^13 + 2*z^12 + 6*z^11 + 2*z^10 + 2*z^9 + 2*z^7 + 2*z^6 + 2*z^5
```

