# $K[x, y]/âŸ¨x - aâ‚, y - aâ‚‚âŸ© â‰Œ K$

Let $P = (aâ‚, aâ‚‚)$ and $ğœ™$ be the evaluation map
$$ ğœ™ : K[x, y] â†’ K $$
$$ ğœ™(f(x, y)) = f(P) $$
then $ğœ™(K) = K$ so we see $ğœ™$ is surjective.

We also see $K[x, y] / \ker ğœ™ â‰Œ K$.
Since the map is surjective, and $K$ is a field, therefore $\ker ğœ™$ is maximal.

Now we prove $\ker ğœ™ = âŸ¨x - aâ‚, y - aâ‚‚âŸ©$. We can easily see
$âŸ¨x - aâ‚, y - aâ‚‚âŸ© âŠ† \ker ğœ™$, so now we prove the reverse inclusion.
We write $f(x, y) = \sum f_i(x)yâ±$ and then see $f(x, aâ‚‚) = \sum f_i(x)aâ‚‚â±$.
$$ f(x, y) - f(x, aâ‚‚) = \sum f_i(x)(yâ± - aâ‚‚â±) $$
but $(yâ± - aâ‚‚â±) = (y - aâ‚‚)(yâ±â»Â¹ + â‹¯ + aâ‚‚)$
$$ â‡’ f(x, y) - f(x, aâ‚‚) âˆˆ âŸ¨y - aâ‚‚âŸ© $$
Continuing with the same argument for $x$, and noting $f(aâ‚, aâ‚‚) = 0$, we see
$$ f(x, y) âˆˆ âŸ¨x - aâ‚, y - aâ‚‚âŸ© â‡’ \ker ğœ™ = âŸ¨x - aâ‚, y - aâ‚‚âŸ© $$

